some morphisms around bisimilarity of streams

NLustre/SemEquiv.v
@@ -13,8 +13,9 @@ Require Import Velus.NLustre.Ordered.
 Require Import Streams.
 
 Require Import Velus.NLustre.NLSemanticsCoIndWire.
-Require Import Velus.NLustre.NLSemanticsCoIndRec.
+Require Import Velus.NLustre.NLSemanticsCoInd.
 
+Require Import Setoid.
 Module Type SEMEQUIV
        (Import Ids   : IDS)
        (Import Op    : OPERATORS)
@@ -23,8 +24,347 @@ Module Type SEMEQUIV
        (Import Syn   : NLSYNTAX  Ids Op Clks)
        (Import Comm  : NLSEMANTICSCOMMON Ids Op OpAux Clks Syn)
        (Import Ord   : ORDERED   Ids Op Clks Syn)
-       (Wire  : NLSEMANTICSCOINDWIRE Ids Op OpAux Clks Syn Comm Ord)
-       (Rec   : NLSEMANTICSCOINDREC  Ids Op OpAux Clks Syn Comm Ord).
+       (Wire         : NLSEMANTICSCOINDWIRE Ids Op OpAux Clks Syn Comm Ord)
+       (Rec          : NLSEMANTICSCOIND Ids Op OpAux Clks Syn Comm Ord).
+
+   Ltac unfold_Stv xs :=
+    rewrite (unfold_Stream xs);
+    destruct xs as [[|]];
+    simpl.
+
+  Ltac unfold_St xs :=
+    rewrite (unfold_Stream xs);
+    destruct xs;
+    simpl.
+
+  Add Parametric Relation A : (Stream A) (@EqSt A)
+      reflexivity proved by (@EqSt_reflex A)
+      symmetry proved by (@sym_EqSt A)
+      transitivity proved by (@trans_EqSt A)
+        as EqStrel.
+
+  Add Parametric Morphism A : (@Cons A)
+      with signature eq ==> @EqSt A ==> @EqSt A
+        as Cons_EqSt.
+  Proof.
+    cofix Cofix.
+    intros x xs xs' Exs.
+    constructor; simpl; auto.
+  Qed.
+
+  Add Parametric Morphism A : (@hd A)
+      with signature @EqSt A ==> eq
+        as hd_EqSt.
+  Proof.
+    intros xs xs' Exs.
+    destruct xs, xs'; inv Exs; simpl; auto.
+  Qed.
+
+  Add Parametric Morphism A : (@tl A)
+      with signature @EqSt A ==> @EqSt A
+        as tl_EqSt.
+  Proof.
+    intros xs xs' Exs.
+    destruct xs, xs'; inv Exs; simpl; auto.
+  Qed.
+
+  Section EqSts.
+    Variable A: Type.
+
+    Definition EqSts (xss yss: list (Stream A)) :=
+      Forall2 (@EqSt A) xss yss.
+
+    Theorem EqSts_reflex: forall xss, EqSts xss xss.
+    Proof.
+      induction xss; constructor; auto.
+      reflexivity.
+    Qed.
+
+    Theorem EqSts_sym: forall xss yss, EqSts xss yss -> EqSts yss xss.
+    Proof.
+      induction xss, yss; intros ** H; auto; try inv H.
+      constructor.
+      - now symmetry.
+      - now apply IHxss.
+    Qed.
+
+    Theorem EqSts_trans: forall xss yss zss, EqSts xss yss -> EqSts yss zss -> EqSts xss zss.
+    Proof.
+      induction xss, yss, zss; intros ** Hx Hy; auto; try inv Hx; try inv Hy.
+      constructor.
+      - now transitivity s.
+      - eapply IHxss; eauto.
+    Qed.
+
+  End EqSts.
+
+  Add Parametric Relation A : (list (Stream A)) (@EqSts A)
+      reflexivity proved by (@EqSts_reflex A)
+      symmetry proved by (@EqSts_sym A)
+      transitivity proved by (@EqSts_trans A)
+        as EqStsrel.
+
+  Add Parametric Morphism A : (@cons (Stream A))
+      with signature @EqSt A ==> @EqSts A ==> @EqSts A
+        as cons_EqSt.
+  Proof. constructor; auto. Qed.
+
+  Add Parametric Morphism
+      A B (P: A -> Stream B -> Prop) xs
+      (P_compat: forall (x: A) (y y': Stream B), y ≡ y' -> (P x y <-> P x y'))
+    : (@Forall2 A (Stream B) P xs)
+      with signature @EqSts B ==> Basics.impl
+        as Forall2_EqSt.
+  Proof.
+    intros ys ys' Eys.
+    revert xs ys ys' Eys;
+      induction xs, ys; intros ** H; inv H; inv Eys; auto.
+    constructor; eauto.  eapply P_compat; eauto.
+    - now symmetry.
+    - eapply IHxs; eauto.
+  Qed.
+
+  Add Parametric Morphism H x : (sem_var H x)
+      with signature @EqSt value ==> Basics.impl
+        as sem_var_EqSt.
+  Proof.
+    intros xs xs' E.
+    intros Sem.
+  Admitted.
+
+  Add Parametric Morphism : merge
+      with signature @EqSt value ==> @EqSt value ==> @EqSt value ==> @EqSt value ==> Basics.impl
+        as merge_EqSt.
+  Proof.
+    cofix Cofix.
+    intros cs cs' Ecs xs xs' Exs ys ys' Eys zs zs' Ezs H.
+    destruct cs' as [[]], xs' as [[]], ys' as [[]], zs' as [[]];
+      inv H; inv Ecs; inv Exs; inv Eys; inv Ezs; simpl in *;
+        try discriminate.
+      + constructor; eapply Cofix; eauto.
+      + rewrite <-H, <-H4, <-H6.
+        constructor; eapply Cofix; eauto.
+      + rewrite <-H, <-H2, <-H6.
+        constructor; eapply Cofix; eauto.
+  Qed.
+
+  Add Parametric Morphism : ite
+      with signature @EqSt value ==> @EqSt value ==> @EqSt value ==> @EqSt value ==> Basics.impl
+        as ite_EqSt.
+  Proof.
+    cofix Cofix.
+    intros es es' Ees ts ts' Ets fs fs' Efs zs zs' Ezs H.
+    destruct es' as [[]], ts' as [[]], fs' as [[]], zs' as [[]];
+      inv H; inv Ees; inv Ets; inv Efs; inv Ezs; simpl in *;
+        try discriminate.
+      + constructor; eapply Cofix; eauto.
+      + rewrite <-H, <-H2, <-H6.
+        constructor; eapply Cofix; eauto.
+      + rewrite <-H, <-H4, <-H6.
+        constructor; eapply Cofix; eauto.
+  Qed.
+
+  Add Parametric Morphism k : (when k)
+      with signature @EqSt value ==> @EqSt value ==> @EqSt value ==> Basics.impl
+        as when_EqSt.
+  Proof.
+    cofix Cofix.
+    intros cs cs' Ecs xs xs' Exs ys ys' Eys H.
+    destruct cs' as [[]], xs' as [[]], ys' as [[]];
+      inv H; inv Ecs; inv Exs; inv Eys; simpl in *;
+        try discriminate.
+      + constructor; eapply Cofix; eauto.
+      + constructor.
+        * eapply Cofix; eauto.
+        * now inv H3.
+      + rewrite <-H, <-H5.
+        constructor.
+        * eapply Cofix; eauto.
+        * now inv H3.
+  Qed.
+
+  Add Parametric Morphism op t : (lift1 op t)
+      with signature @EqSt value ==> @EqSt value ==> Basics.impl
+        as lift1_EqSt.
+  Proof.
+    cofix Cofix.
+    intros es es' Ees ys ys' Eys Lift.
+    destruct es' as [[]], ys' as [[]];
+      inv Lift; inv Eys; inv Ees; simpl in *; try discriminate.
+    - constructor; eapply Cofix; eauto.
+    - constructor.
+      + now inv H1; inv H3.
+      + eapply Cofix; eauto.
+  Qed.
+
+  Add Parametric Morphism op t1 t2 : (lift2 op t1 t2)
+      with signature @EqSt value ==> @EqSt value ==> @EqSt value ==> Basics.impl
+        as lift2_EqSt.
+  Proof.
+    cofix Cofix.
+    intros e1s e1s' Ee1s e2s e2s' Ee2s ys ys' Eys Lift.
+    destruct e1s' as [[]], e2s' as [[]], ys' as [[]];
+      inv Lift; inv Eys; inv Ee1s; inv Ee2s; simpl in *; try discriminate.
+    - constructor; eapply Cofix; eauto.
+    - constructor.
+      + now inv H1; inv H3; inv H5.
+      + eapply Cofix; eauto.
+  Qed.
+
+  Add Parametric Morphism H : (sem_lexp H)
+      with signature @EqSt bool ==> eq ==> @EqSt value ==> Basics.impl
+        as sem_lexp_morph.
+  Proof.
+    intros ** b b' Eb e xs xs' Exs Sem.
+    revert b' xs' Eb Exs; induction Sem.
+    - intros. admit.
+    - econstructor; eauto.
+      eapply sem_var_EqSt; eauto.
+    - econstructor; eauto.
+      apply IHSem; auto; try reflexivity.
+      now rewrite <-Exs.
+    - econstructor.
+      + apply IHSem; auto; reflexivity.
+      + now rewrite <-Exs.
+    - econstructor.
+      + apply IHSem1; auto; reflexivity.
+      + apply IHSem2; auto; reflexivity.
+      + now rewrite <-Exs.
+  Qed.
+
+  Add Parametric Morphism H : (sem_cexp H)
+      with signature @EqSt bool ==> eq ==> @EqSt value ==> Basics.impl
+        as sem_cexp_morph.
+  Proof.
+    intros ** b b' Eb e xs xs' Exs Sem.
+    revert b' xs' Eb Exs; induction Sem.
+    - econstructor; eauto.
+      + apply IHSem1; auto; reflexivity.
+      + apply IHSem2; auto; reflexivity.
+      + now rewrite <-Exs.
+    - econstructor; eauto.
+      + rewrite <-Eb; eauto.
+      + apply IHSem1; auto; reflexivity.
+      + apply IHSem2; auto; reflexivity.
+      + now rewrite <-Exs.
+    - constructor.
+      now rewrite <-Eb, <-Exs.
+  Qed.
+
+  Add Parametric Morphism : Wire.merge_reset
+      with signature @EqSt bool ==> @EqSt bool ==> @EqSt bool
+        as merge_reset_EqSt.
+  Proof.
+    cofix Cofix.
+    intros r1 r1' Er1 r2 r2' Er2.
+    unfold_St r1; unfold_St r1'; unfold_St r2; unfold_St r2'.
+    constructor; inv Er1; inv Er2; simpl in *; auto.
+    now subst.
+  Qed.
+
+  CoFixpoint wire_fby1_EqSt_fix (v c: val)
+           (rs rs': Stream bool) (Ers: rs ≡ rs')
+           (xs xs': Stream value) (Exs: xs ≡ xs') :
+    Wire.fby1 rs v c xs ≡ Wire.fby1 rs' v c xs'
+  with wire_fby_EqSt_fix (c: val)
+                     (rs rs': Stream bool) (Ers: rs ≡ rs')
+                     (xs xs': Stream value) (Exs: xs ≡ xs') :
+         Wire.fby rs c xs ≡ Wire.fby rs' c xs'.
+  Proof.
+    - unfold_Stv rs; unfold_Stv rs'; unfold_Stv xs; unfold_Stv xs';
+        constructor; inv Exs; inv Ers; simpl in *; try discriminate; auto.
+      + inv H; apply wire_fby1_EqSt_fix; auto.
+      + inv H; apply wire_fby1_EqSt_fix; auto.
+    - unfold_Stv xs; unfold_Stv xs'; unfold_St rs; unfold_St rs';
+        constructor; inv Exs; inv Ers; simpl in *; try discriminate; auto.
+      inv H; apply wire_fby1_EqSt_fix; auto.
+  Qed.
+
+  Add Parametric Morphism : Wire.fby
+      with signature @EqSt bool ==> eq ==> @EqSt value ==> @EqSt value
+        as wire_fby_EqSt.
+  Proof. intros; apply wire_fby_EqSt_fix; auto. Qed.
+
+  Add Parametric Morphism : clocks_of
+      with signature @EqSts value ==> @EqSt bool
+        as clocks_of_EqSt.
+  Proof.
+    cofix Cofix.
+    intros xs xs' Exs.
+    constructor; simpl.
+    - clear Cofix.
+      revert dependent xs'.
+      induction xs; intros; try inv Exs; simpl; auto.
+      f_equal; auto.
+      now rewrite H1.
+    - apply Cofix.
+      clear Cofix.
+      revert dependent xs'.
+      induction xs; intros; try inv Exs; simpl; constructor.
+      + now rewrite H1.
+      + now apply IHxs.
+  Qed.
+
+  Fixpoint wire_sem_equation_morph_fix
+           (G: global) (H: history)
+           (b b': Stream bool) (Eb: b ≡ b')
+           (r r': Stream bool) (Er: r ≡ r')
+           (e: equation)
+           (Sem: Wire.sem_equation G H b r e) {struct Sem} :
+    Wire.sem_equation G H b' r' e
+  with wire_sem_node_morph_fix
+         (G: global)
+         (r r': Stream bool) (Er: r ≡ r')
+         (f: ident)
+         (xss xss': list (Stream value)) (Exss: EqSts value xss xss')
+         (yss yss': list (Stream value)) (Eyss: EqSts value yss yss')
+         (Sem: Wire.sem_node G r f xss yss) {struct Sem} :
+    Wire.sem_node G r' f xss' yss'.
+  Proof.
+    - induction Sem.
+      + econstructor; eauto.
+        now rewrite <-Eb.
+      + econstructor; eauto.
+        * apply Forall2_impl_In with (P:=sem_lexp H b); eauto.
+          intros; now rewrite <-Eb.
+        * eapply wire_sem_node_morph_fix; eauto; reflexivity.
+      + econstructor; eauto.
+        * apply Forall2_impl_In with (P:=sem_lexp H b); eauto.
+          intros; now rewrite <-Eb.
+        * eapply wire_sem_node_morph_fix; eauto; try reflexivity.
+          rewrite <-Er; reflexivity.
+      + econstructor; eauto.
+        * rewrite <-Eb; eauto.
+        * subst.
+          eapply sem_var_EqSt; eauto.
+          now rewrite <-Er.
+    - induction Sem.
+      econstructor; eauto.
+      + instantiate (1:=H).
+        eapply Forall2_EqSt; eauto.
+        intros; split; apply sem_var_EqSt; auto.
+        now symmetry.
+      + eapply Forall2_EqSt; eauto.
+        intros; split; apply sem_var_EqSt; auto.
+        now symmetry.
+      + apply Forall_impl with (P:=Wire.sem_equation G H (clocks_of xss) r); auto.
+        apply wire_sem_equation_morph_fix; auto.
+        now rewrite Exss.
+  Admitted.
+
+  Add Parametric Morphism G H : (Wire.sem_equation G H)
+      with signature @EqSt bool ==> @EqSt bool ==> eq ==> Basics.impl
+        as wire_sem_equation_morph.
+  Proof.
+    unfold Basics.impl; apply wire_sem_equation_morph_fix.
+  Qed.
+
+  Add Parametric Morphism G : (Wire.sem_node G)
+      with signature @EqSt bool ==> eq ==> @EqSts value ==> @EqSts value ==> Basics.impl
+        as wire_sem_node_morph.
+  Proof.
+    unfold Basics.impl; apply wire_sem_node_morph_fix.
+  Qed.
 
   CoFixpoint false_s : Stream bool := false ::: false_s.
 
@@ -37,30 +377,30 @@ Module Type SEMEQUIV
 
     Variable G: global.
 
-    Lemma fby1_equiv:
-      forall c v xs ys,
-        Wire.fby1 false_s v (sem_const c) xs ys <->
-        Rec.fby1 v (sem_const c) xs ys.
+    Remark fby1_equiv:
+      forall c v xs,
+        Wire.fby1 false_s v (sem_const c) xs ≡ Rec.fby1 v (sem_const c) xs.
     Proof.
-      split; revert c v xs ys; cofix CoFby1; intros ** Fby1.
-      - rewrite unfold_false_s in Fby1.
-        inversion Fby1; constructor; auto.
-      - rewrite unfold_false_s.
-        inversion Fby1; constructor; auto.
+      cofix; intros.
+      unfold_Stv xs; constructor; simpl; auto.
     Qed.
 
-    Lemma fby_equiv:
-      forall c xs ys,
-        Wire.fby false_s (sem_const c) xs ys <->
-        Rec.fby (sem_const c) xs ys.
+    Corollary fby_equiv:
+      forall c xs,
+        Wire.fby false_s (sem_const c) xs ≡ Rec.fby (sem_const c) xs.
     Proof.
-      split; revert xs ys; cofix CoFby; intros ** Fby.
-      - rewrite unfold_false_s in Fby.
-        inversion_clear Fby; constructor; auto.
-        now apply fby1_equiv.
-      - rewrite unfold_false_s.
-        inversion_clear Fby; constructor; auto.
-        now apply fby1_equiv.
+      cofix; intros.
+      unfold_Stv xs; constructor; simpl; auto.
+      apply fby1_equiv.
+    Qed.
+
+    Remark merge_reset_with_false:
+      forall r, Wire.merge_reset false_s r ≡ r.
+    Proof.
+      cofix; intro.
+      rewrite unfold_false_s.
+      destruct r.
+      constructor; simpl; auto.
     Qed.
 
     (* CoInductive synchronised: Stream value -> Stream value -> Prop := *)
@@ -84,18 +424,6 @@ Module Type SEMEQUIV
     (*     destruct s as [v]; destruct v; simpl; constructor; auto *)
     (*   end. *)
 
-    (* Lemma true_s'_synchronised: *)
-    (*   forall s, synchronised s (Rec.true_s' s). *)
-    (* Proof. prove_synchro. Qed. *)
-
-    (* Lemma once'_synchronised: *)
-    (*   forall s, synchronised s (Rec.once' s). *)
-    (* Proof. *)
-    (*   prove_synchro. *)
-    (*   destruct (c ==b true_val); auto. *)
-    (*   apply true_s'_synchronised. *)
-    (* Qed. *)
-
     (* Lemma when_witness: *)
     (*   forall k xs ys, *)
     (*     synchronised xs ys -> *)
@@ -112,27 +440,15 @@ Module Type SEMEQUIV
     Lemma WireRec_node_reset:
       forall rs f ess oss,
         Wire.sem_node G (Wire.merge_reset false_s (reset_of rs)) f ess oss ->
-        Rec.sem_node G f ess oss ->
+        (* Rec.sem_node G f ess oss -> *)
         Rec.sem_reset G f (reset_of rs) ess oss.
     Proof.
-      intros ** Reset Node.
-      destruct Reset.
-
-      (* assert (exists xss', Forall2 (fun xs xs' => when true xs (Rec.once' (Rec.reset_of rs)) xs') xss xss') *)
-      (*   as (xss' & When_xss). *)
-      (* { clear; induction xss. *)
-      (*   - eexists; eauto. *)
-      (*   - edestruct IHxss. *)
-      (*     edestruct (when_witness true a (Rec.once' (Rec.reset_of rs))). *)
-      (*     admit. *)
-      (*     eexists. *)
-      (*     constructor; eauto. *)
-      (* } *)
-
-      (* assert (exists rs', when true (Rec.reset_of rs) (Rec.once' (Rec.reset_of rs)) rs') *)
-      (*   as (rs' & When_rs) by apply when_witness, once'_synchronised. *)
-
-       econstructor; eauto.
+      intros ** Reset (* Node *).
+      rewrite merge_reset_with_false in Reset.
+      constructor.
+      inv Reset.
+      intro i.
+      econstructor; eauto.
       - econstructor. clear; induction xss.
         + eexists; eauto.
 
